Final bit of cleanup in RGA theory...

src/RGA.thy
@@ -14,18 +14,19 @@ fun interpret_opers :: "('id::linorder, 'v) operation \<Rightarrow> ('id, 'v) el
   "interpret_opers (Delete n)   xs  = delete xs n"
 
 (* Replicated Growable Array Network *)
-locale rga = network_with_ops _ _ _ interpret_opers +
-  assumes insert_flag: "(i, Broadcast, Insert e n) \<in> set (carriers i) \<Longrightarrow> snd (snd e) = False"
-  assumes allowed_insert: "(i, Broadcast, Insert e n) \<in> set (carriers i) \<Longrightarrow> n = None \<or> 
-                            (\<exists>n' n'' v b. n = Some n' \<and> (i, Deliver, Insert (n', v, b) n'') \<sqsubset>\<^sup>i (i, Broadcast, Insert e n))"
-  assumes insert_id_unique: "id1 = id2 \<Longrightarrow> (i, Broadcast, Insert (id1, v1, b1) n1) \<in> set (carriers i) \<Longrightarrow> (j, Broadcast, Insert (id2, v2, b2) n2) \<in> set (carriers j) \<Longrightarrow> v1 = v2 \<and> n1 = n2"
-  assumes allowed_delete: "(i, Broadcast, Delete x) \<in> set (carriers i) \<Longrightarrow> (\<exists>n' v b. (i, Deliver, Insert (x, v, b) n') \<sqsubset>\<^sup>i (i, Broadcast, Delete x))"
+locale rga = network_with_ops _ _ interpret_opers +
+  assumes insert_flag: "Broadcast (Insert e n) \<in> set (history i) \<Longrightarrow> snd (snd e) = False"
+  assumes allowed_insert: "Broadcast (Insert e n) \<in> set (history i) \<Longrightarrow> n = None \<or> 
+                            (\<exists>n' n'' v b. n = Some n' \<and> Deliver (Insert (n', v, b) n'') \<sqsubset>\<^sup>i Broadcast (Insert e n))"
+  assumes insert_id_unique: "id1 = id2 \<Longrightarrow> Broadcast (Insert (id1, v1, b1) n1) \<in> set (history i) \<Longrightarrow> Broadcast (Insert (id2, v2, b2) n2) \<in> set (history j) \<Longrightarrow> v1 = v2 \<and> n1 = n2"
+  assumes allowed_delete: "Broadcast (Delete x) \<in> set (history i) \<Longrightarrow> (\<exists>n' v b. Deliver (Insert (x, v, b) n') \<sqsubset>\<^sup>i Broadcast (Delete x))"
 
 
 lemma (in rga) allowed_delete_deliver:
-  assumes "(i, Deliver, Delete x) \<in> set (carriers i)"
-  shows "\<exists>n' v b. (i, Deliver, Insert (x, v, b) n') \<sqsubset>\<^sup>i (i, Deliver, Delete x)"
-using assms apply -
+  assumes "Deliver (Delete x) \<in> set (history i)"
+    shows "\<exists>n' v b. Deliver (Insert (x, v, b) n') \<sqsubset>\<^sup>i Deliver (Delete x)"
+using assms
+  apply -
   apply(drule delivery_has_a_cause)
   apply clarsimp
   apply(frule no_message_lost[where j=i])
@@ -42,21 +43,14 @@ using assms apply -
 done
 
 lemma (in rga) allowed_delete_deliver_in_set:
-  assumes "(es@[(i, Deliver, Delete m)]) prefix of i"
-  shows   "\<exists>n v b. (i, Deliver, Insert (m, v, b) n) \<in> set es"
-using assms
-  apply -
-  apply(frule_tac x="(i, Deliver, Delete m)" in prefix_to_carriers)
-  apply force
-  apply(frule allowed_delete_deliver)
-  apply clarsimp
-  apply(drule local_order_prefix_closed_last, assumption)
-  apply force
-done
+  assumes "(es@[Deliver (Delete m)]) prefix of i"
+  shows   "\<exists>n v b. Deliver (Insert (m, v, b) n) \<in> set es"
+by(metis (no_types, lifting) Un_insert_right insert_iff list.simps(15) assms
+    local_order_prefix_closed_last rga.allowed_delete_deliver rga_axioms set_append subsetCE prefix_to_carriers)
 
 lemma (in rga) allowed_insert_deliver:
-  assumes "(i, Deliver, Insert e n) \<in> set (carriers i)"
-  shows   "n = None \<or> (\<exists>n' n'' v b. n = Some n' \<and> (i, Deliver, Insert (n', v, b) n'') \<sqsubset>\<^sup>i (i, Deliver, Insert e n))"
+  assumes "Deliver (Insert e n) \<in> set (history i)"
+  shows   "n = None \<or> (\<exists>n' n'' v b. n = Some n' \<and> Deliver (Insert (n', v, b) n'') \<sqsubset>\<^sup>i Deliver (Insert e n))"
 using assms
   apply -
   apply(frule delivery_has_a_cause)
@@ -70,220 +64,135 @@ using assms
   apply clarsimp
   apply(frule no_message_lost[where j=i]) back
   apply(drule broadcast_causal[rotated, where j=i])
-  apply force
-  apply force
+  apply auto
 done
 
 lemma (in rga) allowed_insert_deliver_in_set:
-  assumes "(es@[(i, Deliver, Insert e m)]) prefix of i"
-  shows   "m = None \<or> (\<exists>m' n v b. m = Some m' \<and> (i, Deliver, Insert (m', v, b) n) \<in> set es)"
-using assms
-  apply -
-  apply(frule_tac x="(i, Deliver, Insert e m)" in prefix_to_carriers)
-  apply force
-  apply(frule allowed_insert_deliver)
-  apply(erule disjE)
-  apply force
-  apply clarsimp
-  apply(drule local_order_prefix_closed_last, assumption)
-  apply force
-done
-
-lemma (in rga) allowed_insert_Some_deliver:
-  assumes "(es@[(i, Deliver, Insert e (Some m))]) prefix of i"
-  shows   "\<exists>n v b. (i, Deliver, Insert (m, v, b) n) \<in> set es"
-  using assms allowed_insert_deliver_in_set[where es=es and i=i and e=e and m="Some m"] by force
-
-lemma (in rga) delete_is_not_first_msg:
-  shows "\<not> ([(i, Deliver, Delete n)] prefix of i)"
-  apply (clarsimp simp: prefix_of_carrier_def)
-  apply(subgoal_tac "(i, Deliver, Delete n) \<in> set (carriers i)")
-  apply(drule allowed_delete_deliver)
-  apply clarsimp
-  using carriers_head_lt apply force
-  apply (metis list.set_intros(1))
-done
-
-lemma (in rga) insert_Some_is_not_first_msg:
-  shows "\<not> ([(i, Deliver, Insert e (Some n))] prefix of i)"
-  by (clarsimp, insert allowed_insert_deliver_in_set[where es="[]" and i=i and e=e and m="Some n"], force)
+  assumes "(es@[Deliver (Insert e m)]) prefix of i"
+  shows   "m = None \<or> (\<exists>m' n v b. m = Some m' \<and> Deliver (Insert (m', v, b) n) \<in> set es)"
+by(metis assms Un_insert_right insert_subset list.simps(15) set_append prefix_to_carriers
+    allowed_insert_deliver local_order_prefix_closed_last)
 
 abbreviation (in rga) apply_operations :: "('a, 'b) operation event list \<Rightarrow> ('a, 'b) elt list option" where
   "apply_operations es \<equiv> hb.apply_operations (node_deliver_messages es) []"
 
-lemma (in rga) apply_operations_empty [simp]: "apply_operations [] = Some []"
+lemma (in rga) apply_operations_empty [simp]:
+  shows "apply_operations [] = Some []"
 by auto
 
-lemma (in rga) apply_operations_Broadcast [simp]: "apply_operations (xs @ [(i, Broadcast, m)]) = apply_operations xs"
-by(auto simp add: node_deliver_messages_def)
+lemma (in rga) apply_operations_Broadcast [simp]:
+  shows "apply_operations (xs @ [Broadcast m]) = apply_operations xs"
+by(auto simp add: node_deliver_messages_def map_filter_def)
 
-lemma (in rga) apply_operations_Deliver [simp]: "apply_operations (xs @ [(i, Deliver, m)]) = (apply_operations xs \<bind> interpret_opers m)"
-by(auto simp add: node_deliver_messages_def hb.kleisli_def)
+lemma (in rga) apply_operations_Deliver [simp]:
+  shows "apply_operations (xs @ [Deliver m]) = (apply_operations xs \<bind> \<langle>m\<rangle>)"
+by(auto simp add: node_deliver_messages_def map_filter_def kleisli_def)
 
-definition filter_deliver_inserts :: "_" where
-  "filter_deliver_inserts \<equiv> List.filter (\<lambda>e. case e of (_, Deliver, Insert _ _) \<Rightarrow> True | _ \<Rightarrow> False)"
+definition indices :: "('a, 'b) operation event list \<Rightarrow> 'a list" where
+  "indices xs \<equiv>
+     List.map_filter (\<lambda>x. case x of Deliver (Insert e i) \<Rightarrow> Some (fst e) | _ \<Rightarrow> None) xs"
 
-lemma [simp]: "filter_deliver_inserts [] = []"
-  by (auto simp: filter_deliver_inserts_def)
+lemma indices_Nil [simp]:
+  shows "indices [] = []"
+by(auto simp: indices_def map_filter_def)
 
-lemma [simp]: "filter_deliver_inserts (xs@ys) = (filter_deliver_inserts xs) @ (filter_deliver_inserts ys)"
-  by (auto simp: filter_deliver_inserts_def)
+lemma indices_append [simp]:
+  shows "indices (xs@ys) = indices xs @ indices ys"
+by(auto simp: indices_def map_filter_def)
 
-lemma [simp]: "filter_deliver_inserts [(a, Broadcast, b)] = []"
-  by (auto simp: filter_deliver_inserts_def)
+lemma indices_Broadcast_singleton [simp]:
+  shows "indices [Broadcast b] = []"
+by(auto simp: indices_def map_filter_def)
 
-definition index_elem_inserted :: "_" where
-  "index_elem_inserted \<equiv> map (\<lambda>e. case e of (_, Deliver, Insert (n, _, _) _) \<Rightarrow> n)"
+lemma indices_Deliver_Insert [simp]:
+  shows "indices [Deliver (Insert e n)] = [fst e]"
+by(auto simp: indices_def map_filter_def)
 
-lemma [simp]: "index_elem_inserted [] = []"
-  by (auto simp: index_elem_inserted_def)
+lemma indices_Deliver_Delete [simp]:
+  shows "indices [Deliver (Delete n)] = []"
+by(auto simp: indices_def map_filter_def)
 
-lemma [simp]: "index_elem_inserted (xs@ys) = (index_elem_inserted xs) @ (index_elem_inserted ys)"
-  by (auto simp: index_elem_inserted_def)
-
-lemma [simp]: "index_elem_inserted (filter_deliver_inserts [(i, Deliver, Insert (a, b, c) n)]) = [a]"
-  by (auto simp: index_elem_inserted_def filter_deliver_inserts_def)
-
-lemma [simp]: "index_elem_inserted (filter_deliver_inserts [(i, Deliver, Delete n)]) = []"
-  by (auto simp: index_elem_inserted_def filter_deliver_inserts_def)
-
-lemma (in rga) idx_in_elem_inserted [intro]: "(i, Deliver, Insert (m, v, b) n) \<in> set xs \<Longrightarrow> m \<in> set (index_elem_inserted (filter_deliver_inserts xs))"
-  by (induct xs) (auto simp: index_elem_inserted_def filter_deliver_inserts_def)
+lemma (in rga) idx_in_elem_inserted [intro]:
+  assumes "Deliver (Insert e n) \<in> set xs"
+  shows   "fst e \<in> set (indices xs)"
+using assms by(induction xs, auto simp add: indices_def map_filter_def)
 
 lemma (in rga) apply_opers_idx_elems:
-  assumes "es prefix of i" "apply_operations es = Some xs"
-  shows   "fst ` set xs = set (index_elem_inserted (filter_deliver_inserts es))"
-using assms apply (induct es arbitrary: xs rule: rev_induct)
-apply clarsimp
-apply clarsimp
-apply (case_tac aa)
-apply (erule_tac x=xsa in meta_allE)
-apply force
-apply clarsimp
-apply (subgoal_tac "apply_operations xs = None \<or> (\<exists>ys. apply_operations xs = Some ys)")
-prefer 2
-apply force
-apply (erule disjE)
-apply force
-apply (erule exE)
-apply (erule_tac x=ys in meta_allE)
-apply clarsimp
-apply (case_tac b)
-apply clarsimp
-apply (subgoal_tac "a=i")
-apply clarsimp
-apply (frule allowed_insert_deliver_in_set)
-apply (erule disjE)
-apply clarsimp
-apply force
-apply clarsimp
-(*
-apply (subgoal_tac "\<exists>ys. insert (apply_operations xs) (aa, ab, ba) (Some m') = Some ys")
-prefer 2
-apply (rule insert_no_failure)
-apply clarsimp
-*)
-apply (subgoal_tac "m' \<in> set (index_elem_inserted (filter_deliver_inserts xs))")
-prefer 2                        
-apply force
-(*
-apply force
-*)
-apply (frule insert_preserve_indices')
-apply clarsimp
-apply force
-apply (rule prefix_consistent)
-apply assumption
-apply force
-apply clarsimp
-apply (subgoal_tac "a=i")
-apply clarsimp
-apply (frule allowed_delete_deliver_in_set)
-apply clarsimp
-(*
-apply (subgoal_tac "\<exists>ys. delete (apply_operations xs) x2 = Some ys")
-apply clarsimp
-*)
-apply (frule delete_preserve_indices)
-apply clarsimp
-apply (subgoal_tac "xs prefix of i")
-apply force
-apply force
-(*
-apply (rule delete_no_failure)
-apply force
-*)
-apply (rule prefix_consistent)
-apply assumption
-apply force
+  assumes "es prefix of i"
+      and "apply_operations es = Some xs"
+    shows "fst ` set xs = set (indices es)"
+using assms
+  apply(induction es arbitrary: xs rule: rev_induct; clarsimp)
+  apply(case_tac x; clarsimp)
+  apply blast
+  apply(case_tac "x2"; clarsimp)
+  apply(auto split: bind_splits)
+  apply(metis (no_types, hide_lams) Un_insert_right image_eqI insert_iff insert_preserve_indices
+        option.sel prefix_of_appendD prod.sel(1) sup_bot.comm_neutral)
+  apply(metis Un_insert_right fst_conv insert_iff insert_preserve_indices option.sel)
+  apply(metis (no_types, hide_lams) Un_insert_right insert_iff insert_preserve_indices' option.sel
+        prefix_of_appendD sup_bot.comm_neutral)
+  apply(metis delete_preserve_indices fst_conv image_eqI prefix_of_appendD)
+  using delete_preserve_indices apply blast
 done
-
 
 lemma (in rga) insert_in_apply_set:
-  assumes "es @ [(i, Deliver, Insert e (Some a))] prefix of i"
-          "(i, Deliver, Insert (a, v, b) n) \<in> set es" "apply_operations es = Some s"
-  shows   "\<exists>v b. (a, v, b) \<in> set s"
-using assms
-apply (case_tac e)
-apply clarsimp
-apply (drule idx_in_elem_inserted)
-apply (subst (asm) apply_opers_idx_elems[symmetric])
-apply force
-apply force
-apply force
-done
+  assumes "es @ [Deliver (Insert e (Some a))] prefix of i"
+      and "Deliver (Insert e' n) \<in> set es"
+      and "apply_operations es = Some s"
+    shows "fst e' \<in> fst ` set s"
+using assms apply_opers_idx_elems idx_in_elem_inserted prefix_of_appendD by blast
 
 lemma (in rga) Insert_no_failure:
-  assumes "es @ [(i, Deliver, Insert e n)] prefix of i"  "apply_operations es = Some s"
-  shows "\<exists>ys. insert s e n = Some ys"
-  using assms apply -
-  apply (frule allowed_insert_deliver_in_set)
-  apply (case_tac n)
-  apply clarsimp
-  apply clarsimp
-  apply (rule insert_no_failure)
-  apply clarsimp
-  using insert_in_apply_set apply (metis idx_in_elem_inserted prefix_of_appendD rga.apply_opers_idx_elems rga_axioms)
-done
+  assumes "es @ [Deliver (Insert e n)] prefix of i" 
+      and "apply_operations es = Some s"
+    shows "\<exists>ys. insert s e n = Some ys"
+by(metis allowed_insert_deliver_in_set assms fst_conv insert_in_apply_set insert_no_failure)
 
 lemma (in rga) delete_no_failure:
-  assumes "es @ [(i, Deliver, Delete n)] prefix of i" "apply_operations es = Some s"
-  shows   "\<exists>ys. delete s n = Some ys"
-  using assms apply -
-  apply (frule allowed_delete_deliver_in_set)
+  assumes "es @ [Deliver (Delete n)] prefix of i"
+      and "apply_operations es = Some s"
+    shows "\<exists>ys. delete s n = Some ys"
+using assms 
+  apply -
+  apply(frule allowed_delete_deliver_in_set)
   apply clarsimp
-  apply (rule delete_no_failure)
-  apply (drule idx_in_elem_inserted)
-  apply (subst (asm) apply_opers_idx_elems[symmetric])
-  apply force
-  apply force
-  apply force
+  apply(rule delete_no_failure)
+  apply(drule idx_in_elem_inserted)
+  apply(auto simp add: apply_opers_idx_elems)
 done
 
 lemma (in rga) Insert_equal:
   assumes "fst e1 = fst e2"
-          "(i, Broadcast, Insert e1 n1) \<in> set (carriers i)"
-          "(j, Broadcast, Insert e2 n2) \<in> set (carriers j)"
-  shows   "Insert e1 n1 = Insert e2 n2"
+      and "Broadcast (Insert e1 n1) \<in> set (history i)"
+      and "Broadcast (Insert e2 n2) \<in> set (history j)"
+    shows "Insert e1 n1 = Insert e2 n2"
 using assms
-  apply (subgoal_tac "e1 = e2")
-  apply (metis surjective_pairing insert_id_unique)
-  apply (cases e1, cases e2; clarsimp)
-  apply (metis insert_flag snd_conv insert_id_unique)
+  apply(subgoal_tac "e1 = e2")
+  apply(metis surjective_pairing insert_id_unique)
+  apply(cases e1, cases e2; clarsimp)
+  apply(metis insert_flag snd_conv insert_id_unique)
 done
+
+lemma (in rga) insert_id_unique_node:
+  assumes "fst e1 = fst e2" 
+      and "Broadcast (Insert e1 n1) \<in> set (history i)"
+      and "Broadcast (Insert e2 n2) \<in> set (history j)"
+    shows "i = j"
+by(metis assms Insert_equal network.broadcasts_unique network_axioms)
 
 lemma (in rga) same_insert:
   assumes "fst e1 = fst e2"
-          "xs prefix of i"
-          "(Insert e1 n1) \<in> set (node_deliver_messages xs)"
-          "(Insert e2 n2) \<in> set (node_deliver_messages xs)"
-  shows   "Insert e1 n1 = Insert e2 n2"
+      and "xs prefix of i"
+      and "(Insert e1 n1) \<in> set (node_deliver_messages xs)"
+      and "(Insert e2 n2) \<in> set (node_deliver_messages xs)"
+    shows "Insert e1 n1 = Insert e2 n2"
 using assms
   apply -
-  apply(subgoal_tac "(i, Deliver, Insert e1 n1) \<in> set (carriers i)")
-  apply(subgoal_tac "(i, Deliver, Insert e2 n2) \<in> set (carriers i)")
-  apply(subgoal_tac "\<exists>j. (j, Broadcast, Insert e1 n1) \<in> set (carriers j)")
-  apply(subgoal_tac "\<exists>j. (j, Broadcast, Insert e2 n2) \<in> set (carriers j)")
+  apply(subgoal_tac "Deliver (Insert e1 n1) \<in> set (history i)")
+  apply(subgoal_tac "Deliver (Insert e2 n2) \<in> set (history i)")
+  apply(subgoal_tac "\<exists>j. Broadcast (Insert e1 n1) \<in> set (history j)")
+  apply(subgoal_tac "\<exists>j. Broadcast (Insert e2 n2) \<in> set (history j)")
   apply(erule exE)+
   apply(rule Insert_equal, force, force, force) 
   apply(simp add: delivery_has_a_cause)
@@ -291,226 +200,153 @@ using assms
   apply(simp add: node_deliver_messages_def prefix_msg_in_history)+
 done
 
-lemma (in rga) insert_id_unique_node:
-  assumes "fst e1 = fst e2" 
-          "(i, Broadcast, Insert e1 n1) \<in> set (carriers i)"
-          "(j, Broadcast, Insert e2 n2) \<in> set (carriers j)"
-  shows   "i = j"
-  using assms broadcasts_unique insert_id_unique
-  by (smt insert_flag prod.collapse)
-
 lemma (in rga) insert_commute_assms:
-  assumes "{(i, Deliver, Insert e n), (i, Deliver, Insert e' n')} \<subseteq> set (carriers i)"
-     and  "hb.concurrent (Insert e n) (Insert e' n')"
- shows    "n = None \<or> n \<noteq> Some (fst e')"
+  assumes "{Deliver (Insert e n), Deliver (Insert e' n')} \<subseteq> set (history i)"
+      and "hb.concurrent (Insert e n) (Insert e' n')"
+    shows "n = None \<or> n \<noteq> Some (fst e')"
 using assms
-apply (clarsimp simp: hb_def hb.concurrent_def)
-apply (case_tac e')
-apply clarsimp
-apply (frule delivery_has_a_cause)
-apply (frule delivery_has_a_cause) back
-apply clarsimp
-apply (frule allowed_insert)
-apply clarsimp
-apply (erule_tac x=j in allE) back
-apply clarsimp
-apply (subgoal_tac "(j, Deliver, Insert (a, v, ba) n'') = (j, Deliver, Insert (a, b, c) n')")
-apply clarsimp
-using insert_id_unique 
-by (smt delivery_has_a_cause rga.insert_flag rga_axioms insert_subset local_order_carrier_closed prod.sel(2))
-
-lemma (in rga) Insert_Insert_concurrent: 
-  assumes "{(i, Deliver, Insert (n, v, b) k), (i, Deliver, Insert e (Some m))} \<subseteq> set (carriers i)"
-     and  "hb.concurrent (Insert (n, v, b) k) (Insert e (Some m))"
- shows    "n \<noteq> m"
-using assms
-apply -
-apply (insert insert_commute_assms[of i e "Some m" "(n, v, b)" k])
-apply auto
+  apply(clarsimp simp: hb_def hb.concurrent_def)
+  apply(case_tac e')
+  apply clarsimp
+  apply(frule delivery_has_a_cause)
+  apply(frule delivery_has_a_cause) back
+  apply clarsimp
+  apply(frule allowed_insert)
+  apply clarsimp
+  apply(erule_tac x=j in allE) back
+  apply clarsimp
+  apply(subgoal_tac "(j, Deliver, Insert (a, v, ba) n'') = (j, Deliver, Insert (a, b, c) n')")
+  apply clarsimp
+  using insert_id_unique apply (smt delivery_has_a_cause rga.insert_flag rga_axioms insert_subset local_order_carrier_closed prod.sel(2))
 done
+
+lemma (in rga) Insert_Insert_concurrent:
+  assumes "{Deliver (Insert e k), Deliver (Insert e' (Some m))} \<subseteq> set (history i)"
+      and "hb.concurrent (Insert e k) (Insert e' (Some m))"
+    shows "fst e \<noteq> m"
+by(metis (no_types, hide_lams) hb.concurrent_comm insert_commute insert_commute_assms option.simps(3) assms)
 
 lemma (in rga) insert_valid_assms:
- assumes "(i, Deliver, Insert e n) \<in> set (carriers i)"
- shows    "n = None \<or> n \<noteq> Some (fst e)"
-using assms
-  apply(subgoal_tac "\<exists>j. (j, Broadcast, Insert e n) \<in> set (carriers j)")
-  apply(erule exE)
-  apply(drule allowed_insert[rotated])
-  apply(erule disjE)
-  apply force
-  apply clarsimp
-  apply(metis Insert_equal broadcast_causal delivery_has_a_cause fst_conv insert_subset local_order_carrier_closed node_total_order_irrefl)
-  apply(simp add: delivery_has_a_cause)
-done
+ assumes "Deliver (Insert e n) \<in> set (history i)"
+   shows "n = None \<or> n \<noteq> Some (fst e)"
+using assms by(meson allowed_insert_deliver hb.concurrent_def hb.less_asym insert_subset local_order_carrier_closed rga.insert_commute_assms rga_axioms)
 
 lemma (in rga) Insert_Delete_concurrent:
-  assumes "{(i, Deliver, Insert e n), (i, Deliver, Delete n')} \<subseteq> set (carriers i)"
-     and  "hb.concurrent (Insert e n) (Delete n')"
- shows    "n' \<noteq> fst e"
-using assms
-apply (clarsimp simp: hb_def hb.concurrent_def)
-apply (drule delivery_has_a_cause)
-apply (drule delivery_has_a_cause)
-apply clarsimp
-apply (drule allowed_delete)
-apply clarsimp
-apply (erule_tac x=ja in allE)
-apply clarsimp
-apply(subgoal_tac "(ja, Broadcast, Insert (fst e, v, b) n'a) = (j, Broadcast, Insert e n)")
-apply clarsimp
-apply (case_tac e)
-apply clarsimp
-apply (subgoal_tac "j = ja")
-apply clarsimp
-apply (smt delivery_has_a_cause rga.insert_flag rga_axioms insert_id_unique insert_subset local_order_carrier_closed prod.sel(2))
-using insert_id_unique_node
-by (smt delivery_has_a_cause insert_flag insert_id_unique insert_subset local_order_carrier_closed prod.sel(2))
+  assumes "{Deliver (Insert e n), Deliver (Delete n')} \<subseteq> set (history i)"
+      and "hb.concurrent (Insert e n) (Delete n')"
+    shows "n' \<noteq> fst e"
+using assms by(metis Insert_equal allowed_delete delivery_has_a_cause fst_conv hb.concurrent_def hb_def insert_subset local_order_carrier_closed)
 
 lemma (in rga) node_deliver_messages_distinct:
   assumes "xs prefix of i"
   shows "distinct (node_deliver_messages xs)"
 using assms
-  apply (induct xs rule: rev_induct)
+  apply(induction xs rule: rev_induct)
   apply simp
-  apply (clarsimp simp add: node_deliver_messages_append)
+  apply(clarsimp simp add: node_deliver_messages_append)
   apply safe
   apply force
-  apply (clarsimp simp: node_deliver_messages_def)
+  apply(clarsimp simp: node_deliver_messages_def map_filter_def)
   apply clarsimp
-  apply (frule prefix_distinct)
+  apply(frule prefix_distinct)
   apply clarsimp
-  apply (subst (asm) node_deliver_messages_def) back back back
-  apply clarsimp
-  apply (case_tac aa; clarsimp)
-  apply (subst (asm) node_deliver_messages_def) back
-  apply clarsimp
-  apply (case_tac ab; clarsimp)
-  apply (subgoal_tac "a=i")
-  apply (subgoal_tac "aa=i")
-  apply clarsimp
-  apply (rule_tac b=Deliver and c=ba in prefix_consistent)
-  apply assumption
-  apply force
-  apply (rule_tac b=Deliver and c=ba in prefix_consistent)
-  apply assumption
-  apply force
+  apply(subst (asm) node_deliver_messages_def) back back back
+  apply(clarsimp simp add: map_filter_def)
+  apply(case_tac x; clarsimp)
+  apply(subst (asm) node_deliver_messages_def) back
+  apply(clarsimp simp add: map_filter_def)
+  apply(case_tac x; clarsimp)
 done
 
-lemma (in rga) deliver_delete_neq_head:
-  shows "carriers i \<noteq> (i, Deliver, Delete e)#ys"
-  apply clarsimp
-  apply(subgoal_tac "(i, Deliver, Delete e) \<in> set (carriers i)")
-  apply(drule sym)
-  apply(frule delivery_has_a_cause)
-  apply clarsimp
-  apply(drule allowed_delete)
-  apply clarsimp
-  apply(frule local_order_carrier_closed)
-  apply clarsimp
-  apply(drule delivery_has_a_cause) back
-  apply clarsimp
-  apply(frule no_message_lost[where j=i]) back
-  apply(drule broadcast_causal[rotated, where j=i])
-  apply force
-  using carriers_head_lt apply blast
-  apply force
-done
-
-corollary (in rga) hb_consistent_prefix:
+lemma (in rga) hb_consistent_prefix:
   assumes "xs prefix of i"
-  shows   "hb.hb_consistent (node_deliver_messages xs)"
+    shows "hb.hb_consistent (node_deliver_messages xs)"
 using assms
-apply (clarsimp simp: prefix_of_carrier_def)
-apply (rule_tac i=i in hb_consistent_technical)
-apply (subst carriers_compatible)
-apply(subgoal_tac "xs = [] \<or> (\<exists>c. xs = [c]) \<or> (length (xs) > 1)")
-apply (erule disjE)
-apply clarsimp
-apply (erule disjE)
-apply clarsimp
-apply (drule list_nth_split)
-apply assumption
-apply clarsimp
-apply clarsimp
-apply (rule_tac x=xsa in exI)
-apply (rule_tac x=ysa in exI)
-apply (rule_tac x="zs@ys" in exI)
-apply (metis Cons_eq_appendI append_assoc)
-apply force
+  apply(clarsimp simp: prefix_of_node_history_def)
+  apply(rule_tac i=i in hb_consistent_technical)
+  apply(subst history_order_def)
+  apply(subgoal_tac "xs = [] \<or> (\<exists>c. xs = [c]) \<or> (length (xs) > 1)")
+  apply(erule disjE)
+  apply clarsimp
+  apply(erule disjE)
+  apply clarsimp
+  apply(drule list_nth_split)
+  apply assumption
+  apply clarsimp
+  apply clarsimp
+  apply(rule_tac x=xsa in exI)
+  apply(rule_tac x=ysa in exI)
+  apply(rule_tac x="zs@ys" in exI)
+  apply(metis Cons_eq_appendI append_assoc)
+  apply force
 done
-
-(*
-lemma (in rga) rewrite: "\<langle>x\<rangle> \<rhd> (\<langle>y\<rangle> \<rhd> (Some xs)) = do { ys \<leftarrow> \<langle>y\<rangle> (Some xs); \<langle>x\<rangle> (Some ys) }"
-apply (case_tac "\<langle>y\<rangle> (Some xs)")
-apply auto
-done
-*)
 
 lemma (in rga) concurrent_operations_commute:
   assumes "xs prefix of i"
   shows "hb.concurrent_ops_commute (node_deliver_messages xs)"
 using assms
-apply (clarsimp simp: hb.concurrent_ops_commute_def)
-apply (rule ext)
-apply(unfold hb.kleisli_def)
-apply (case_tac x; case_tac y)
-apply clarsimp
-apply (case_tac "a = ab")
-apply (subgoal_tac "(a, aa, b) = (ab, ac, ba) \<and> x12a = x12")
-apply force
-defer
-apply(subgoal_tac "Ordered_List.insert xa (a, aa, b) x12 \<bind> (\<lambda>x. Ordered_List.insert x (ab, ac, ba) x12a) = Ordered_List.insert xa (ab, ac, ba) x12a \<bind> (\<lambda>x. Ordered_List.insert x (a, aa, b) x12)")
-apply(metis (no_types, lifting) Option.bind_cong interpret_opers.simps(1))
-apply (rule insert_commutes)
-apply simp
-prefer 2
-apply (subst (asm) hb.concurrent_comm)
-apply (rule insert_commute_assms)
-prefer 2
-apply assumption
-apply clarsimp
-apply (rule conjI)
-apply (rule prefix_msg_in_history, assumption, force)
-apply (rule prefix_msg_in_history, assumption, force)
-apply (rule insert_commute_assms)
-prefer 2
-apply assumption
-apply clarsimp
-apply (rule conjI)
-apply (rule prefix_msg_in_history, assumption, force)
-apply (rule prefix_msg_in_history, assumption, force)
-apply(clarsimp simp del: delete.simps)
-apply(subgoal_tac "Ordered_List.insert xa (a, aa, b) x12 \<bind> (\<lambda>x. Ordered_List.delete x x2) = delete xa x2 \<bind> (\<lambda>x. Ordered_List.insert x (a, aa, b) x12)")
-apply(metis (no_types, lifting) Option.bind_cong interpret_opers.simps)
-apply (rule insert_delete_commute)
-apply (rule insert_valid_assms)
-using prefix_msg_in_history apply blast
-apply (rule Insert_Delete_concurrent)
-apply clarsimp
-using prefix_msg_in_history apply blast
-apply(clarsimp)
-apply(clarsimp simp del: delete.simps)
-apply(subgoal_tac "delete xa x2 \<bind> (\<lambda>x. insert x (a, aa, b) x12) = Ordered_List.insert xa (a, aa, b) x12 \<bind> (\<lambda>x. delete x x2)")
-apply(metis (no_types, lifting) Option.bind_cong interpret_opers.simps)
-apply (rule insert_delete_commute[symmetric])
-apply (rule insert_valid_assms)
-using prefix_msg_in_history apply blast
-apply (rule Insert_Delete_concurrent)
-using prefix_msg_in_history apply blast
-apply (subst (asm) hb.concurrent_comm)
-apply assumption
-apply(clarsimp simp del: delete.simps)
-apply(subgoal_tac "delete xa x2 \<bind> (\<lambda>x. delete x x2a) = delete xa x2a \<bind> (\<lambda>x. delete x x2)")
-apply (metis (mono_tags, lifting) Option.bind_cong interpret_opers.simps(2))
-apply (rule delete_commutes)
-using same_insert apply force
+  apply(clarsimp simp: hb.concurrent_ops_commute_def)
+  apply(rule ext)
+  apply(unfold kleisli_def)
+  apply(case_tac x; case_tac y)
+  apply clarsimp
+  apply(case_tac "a = ab")
+  apply(subgoal_tac "(a, aa, b) = (ab, ac, ba) \<and> x12a = x12")
+  apply force
+  defer
+  apply(subgoal_tac "Ordered_List.insert xa (a, aa, b) x12 \<bind> (\<lambda>x. Ordered_List.insert x (ab, ac, ba) x12a) = Ordered_List.insert xa (ab, ac, ba) x12a \<bind> (\<lambda>x. Ordered_List.insert x (a, aa, b) x12)")
+  apply(metis (no_types, lifting) Option.bind_cong interpret_opers.simps(1))
+  apply(rule insert_commutes)
+  apply simp
+  prefer 2
+  apply(subst (asm) hb.concurrent_comm)
+  apply(rule insert_commute_assms)
+  prefer 2
+  apply assumption
+  apply clarsimp
+  apply(rule conjI)
+  apply(rule prefix_msg_in_history, assumption, force)
+  apply(rule prefix_msg_in_history, assumption, force)
+  apply(rule insert_commute_assms)
+  prefer 2
+  apply assumption
+  apply clarsimp
+  apply(rule conjI)
+  apply(rule prefix_msg_in_history, assumption, force)
+  apply(rule prefix_msg_in_history, assumption, force)
+  apply(clarsimp simp del: delete.simps)
+  apply(subgoal_tac "Ordered_List.insert xa (a, aa, b) x12 \<bind> (\<lambda>x. Ordered_List.delete x x2) = delete xa x2 \<bind> (\<lambda>x. Ordered_List.insert x (a, aa, b) x12)")
+  apply(metis (no_types, lifting) Option.bind_cong interpret_opers.simps)
+  apply(rule insert_delete_commute)
+  apply(rule insert_valid_assms)
+  using prefix_msg_in_history apply blast
+  apply(rule Insert_Delete_concurrent)
+  apply clarsimp
+  using prefix_msg_in_history apply blast
+  apply(clarsimp)
+  apply(clarsimp simp del: delete.simps)
+  apply(subgoal_tac "delete xa x2 \<bind> (\<lambda>x. insert x (a, aa, b) x12) = Ordered_List.insert xa (a, aa, b) x12 \<bind> (\<lambda>x. delete x x2)")
+  apply(metis (no_types, lifting) Option.bind_cong interpret_opers.simps)
+  apply(rule insert_delete_commute[symmetric])
+  apply(rule insert_valid_assms)
+  using prefix_msg_in_history apply blast
+  apply(rule Insert_Delete_concurrent)
+  using prefix_msg_in_history apply blast
+  apply(subst (asm) hb.concurrent_comm)
+  apply assumption
+  apply(clarsimp simp del: delete.simps)
+  apply(subgoal_tac "delete xa x2 \<bind> (\<lambda>x. delete x x2a) = delete xa x2a \<bind> (\<lambda>x. delete x x2)")
+  apply(metis (mono_tags, lifting) Option.bind_cong interpret_opers.simps(2))
+  apply(rule delete_commutes)
+  using same_insert apply force
 done
 
-corollary (in rga) main_result_of_paper:
+corollary (in rga) rga_convergence:
   assumes "set (node_deliver_messages xs) = set (node_deliver_messages ys)"
-          "xs prefix of i"
-          "ys prefix of j"
-  shows  "apply_operations xs = apply_operations ys"
-using assms by(auto intro: hb.convergence_ext concurrent_operations_commute node_deliver_messages_distinct hb_consistent_prefix)
+      and "xs prefix of i"
+      and "ys prefix of j"
+    shows "apply_operations xs = apply_operations ys"
+using assms by(auto intro: hb.convergence_ext concurrent_operations_commute
+                node_deliver_messages_distinct hb_consistent_prefix)
 
 end
